chore: rename shiftLeft to shiftLeftConst

LeanSAT/Reflect/BVExpr/Basic.lean
@@ -57,23 +57,23 @@ inductive BVUnOp where
 -- shifting is "unary" because we only allow shifting by constant values for now.
 -- for shift by arbitrary values we would need to implement and verify something like a barell
 -- shifter
-| shiftLeft (n : Nat)
+| shiftLeftConst (n : Nat)
 
 namespace BVUnOp
 
 def toString : BVUnOp → String
   | not => "~"
-  | shiftLeft n => s!"<< {n}"
+  | shiftLeftConst n => s!"<< {n}"
 
 instance : ToString BVUnOp := ⟨toString⟩
 
 def eval : BVUnOp → (BitVec w → BitVec w)
   | not => (~~~ ·)
-  | shiftLeft n => (· <<< n)
+  | shiftLeftConst n => (· <<< n)
 
 @[simp] theorem eval_not : eval .not = ((~~~ ·) : BitVec w → BitVec w) := by rfl
 @[simp]
-theorem eval_shiftLeft : eval (.shiftLeft n) = ((· <<< n) : BitVec w → BitVec w) := by
+theorem eval_shiftLeftConst : eval (shiftLeftConst n) = ((· <<< n) : BitVec w → BitVec w) := by
   rfl
 
 end BVUnOp
